wps for client half of marshalling Get helpers

src/program_proof/memkv/memkv_marshal_get_proof.v
@@ -1,6 +1,7 @@
 From Perennial.program_proof Require Import proof_prelude.
 From Goose.github_com.mit_pdos.gokv Require Import memkv.
 From Perennial.goose_lang Require Import ffi.grove_ffi.
+From Perennial.program_proof Require Import marshal_proof.
 
 (*
   Defines Coq request and reply types for shard server Get RPC. Also defines
@@ -32,29 +33,64 @@ Definition own_GetReply reply_ptr rep : iProp Σ :=
   ∃ val_sl,
   "HErr" ∷ reply_ptr ↦[GetReply.S :: "Err"] #rep.(GR_Err) ∗
   "HValue" ∷ reply_ptr ↦[GetReply.S :: "Value"] (slice_val val_sl) ∗
-  "HValue_sl" ∷ typed_slice.is_slice val_sl byteT 1%Qp rep.(GR_Value)
+  "HValue_sl" ∷ ∃ (q:Qp), (typed_slice.is_slice_small val_sl byteT q rep.(GR_Value))
 .
 
-Axiom has_encoding_GetRequest : (list u8) → GetRequestC → Prop.
-Axiom has_encoding_GetReply : (list u8) → GetReplyC → Prop.
+Definition has_encoding_GetRequest (data:list u8) (args:GetRequestC) :=
+  has_encoding data [ EncUInt64 args.(GR_CID) ; EncUInt64 args.(GR_Seq) ; EncUInt64 args.(GR_Key) ].
 
-Lemma wp_encodeGetRequest (cid seq key:u64) :
+Definition has_encoding_GetReply (data:list u8) (rep:GetReplyC) :=
+  has_encoding data [ EncUInt64 rep.(GR_Err) ; EncUInt64 (length rep.(GR_Value)) ; EncBytes rep.(GR_Value) ].
+
+Lemma wp_encodeGetRequest args_ptr args :
   {{{
-       True
+       own_GetRequest args_ptr args
   }}}
-    encodeGetRequest (#cid, (#seq, (#key, #())))%V
+    encodeGetRequest #args_ptr
   {{{
-       (reqData:list u8) req_sl, RET (slice_val req_sl); ⌜has_encoding_GetRequest reqData {| GR_CID:=cid; GR_Seq:=seq; GR_Key:=key |}⌝ ∗
+       (reqData:list u8) req_sl, RET (slice_val req_sl); ⌜has_encoding_GetRequest reqData args⌝ ∗
                                                typed_slice.is_slice req_sl byteT 1%Qp reqData
   }}}.
 Proof.
-Admitted.
+  iIntros (Φ) "Hpre HΦ".
+  iNamed "Hpre".
+  wp_lam.
+  wp_apply (wp_new_enc).
+  iIntros (?) "Henc".
+  wp_pures.
+
+  wp_loadField.
+  wp_apply (wp_Enc__PutInt with "[$Henc]").
+  { done. }
+  iIntros "Henc".
+  wp_pures.
+
+  wp_loadField.
+  wp_apply (wp_Enc__PutInt with "[$Henc]").
+  { done. }
+  iIntros "Henc".
+  wp_pures.
+
+  wp_loadField.
+  wp_apply (wp_Enc__PutInt with "[$Henc]").
+  { done. }
+  iIntros "Henc".
+  wp_pures.
+
+  wp_apply (wp_Enc__Finish with "[$Henc]").
+  iIntros (??) "(%Henc & Hlen & Hsl)".
+  iApply "HΦ".
+  iFrame.
+  done.
+Qed.
 
 Lemma has_encoding_GetRequest_inj (reqRaw:list u8) req req' :
   has_encoding_GetRequest reqRaw req →
   has_encoding_GetRequest reqRaw req' →
   req = req'.
 Proof.
+  intros.
+  unfold has_encoding_GetRequest in *.
 Admitted.
 
 Lemma wp_decodeGetReply rep rep_sl repData :
@@ -64,12 +100,43 @@ Lemma wp_decodeGetReply rep rep_sl repData :
   }}}
     decodeGetReply (slice_val rep_sl)
   {{{
-       (rep_ptr:loc) val_sl, RET #rep_ptr;
-       rep_ptr ↦[GetReply.S :: "Err"] #rep.(GR_Err) ∗
-       rep_ptr ↦[GetReply.S :: "Value"] (slice_val val_sl) ∗
-       typed_slice.is_slice val_sl byteT 1%Qp rep.(GR_Value)
+       (rep_ptr:loc) , RET #rep_ptr;
+       own_GetReply rep_ptr rep
   }}}.
 Proof.
+  iIntros (Φ) "[Hsl %Henc] HΦ".
+  wp_lam.
+  wp_apply (wp_allocStruct).
+  { unfold GetReply.S. simpl.
+    unfold ErrorType. admit. }
+  iIntros (rep_ptr) "Hrep".
+  iDestruct (struct_fields_split with "Hrep") as "HH".
+  iNamed "HH".
+  wp_pures.
+  iDestruct (typed_slice.is_slice_small_acc with "Hsl") as "[Hsl Hsl_close]".
+  wp_apply (wp_new_dec with "[$Hsl]").
+  { done. }
+  iIntros (?) "Hdec".
+  wp_pures.
+
+  wp_apply (wp_Dec__GetInt with "[$Hdec]").
+  iIntros "Hdec".
+  wp_storeField.
+
+  wp_apply (wp_Dec__GetInt with "[$Hdec]").
+  iIntros "Hdec".
+  wp_apply (wp_Dec__GetBytes with "[$Hdec]").
+  { admit. } (* TODO: make a "safe_size_sl" predicate and keep it everywhere *)
+  iIntros (??) "[Hsl Hdec]".
+  wp_apply (wp_storeField with "Value").
+  { apply slice_val_ty. }
+  iIntros "Value".
+  wp_pures.
+  iApply "HΦ".
+  iModIntro.
+  iExists _.
+  iFrame.
+  iExists _; iFrame.
 Admitted.
 
 End memkv_marshal_get_proof.
